theories/iris/wp_codegen.v
@@ -2,10 +2,10 @@ Require Import iris.proofmode.tactics.
 
 Require Import Wasm.iris.rules.iris_rules.
 
-Require Import RichWasm.term.
+From RichWasm Require Import term typing.
 Require Import RichWasm.iris.gc.
-Require Import RichWasm.iris.logrel.relations.
-From RichWasm.compiler Require Import codegen instrs util.
+From RichWasm.iris.logrel Require Import relations util.
+From RichWasm.compiler Require Import codegen instrs types util.
 
 Set Bullet Behavior "Strict Subproofs".
 Set Default Goal Selector "!".
@@ -27,10 +27,10 @@ Section CodeGen.
     run_codegen c2 wl1 = inr (y, wl', es2) /\
     ⊢ ↪[frame] f -∗
       ((⌜i <> Wasm_int.int_zero i32m⌝ ∧
-        ▷ (↪[frame] f -∗ WP [AI_basic (BI_block tf es1)] @ s; E {{ w, Φ w }})) ∨
+        ▷ (↪[frame] f -∗ WP [AI_basic (BI_block tf es1)] @ s; E {{ v, Φ v }})) ∨
        (⌜i = Wasm_int.int_zero i32m⌝ ∧
-        ▷ (↪[frame] f -∗ WP [AI_basic (BI_block tf es2)] @ s; E {{ w, Φ w }}))) -∗
-      WP to_e_list (BI_const (VAL_int32 i) :: es) @ s; E {{ w, Φ w }}.
+        ▷ (↪[frame] f -∗ WP [AI_basic (BI_block tf es2)] @ s; E {{ v, Φ v }}))) -∗
+      WP to_e_list (BI_const (VAL_int32 i) :: es) @ s; E {{ v, Φ v }}.
   Proof.
     intros Hcomp.
     unfold if_c in Hcomp.
@@ -77,11 +77,12 @@ Section CodeGen.
       interp_val sr [RefT cap (LocP ptr GCMem) ht] (immV [VAL_int32 i]) ∨
       interp_val sr [RefT cap (LocP ptr LinMem) ht] (immV [VAL_int32 i]) -∗
       ▷ (↪[frame] f -∗
-         (interp_val sr [RefT cap (LocP ptr GCMem) ht] (immV [VAL_int32 i]) -∗
-          WP [AI_basic (BI_block tf es2)] @ s; E {{ w, Φ w }}) ∨
-         (interp_val sr [RefT cap (LocP ptr LinMem) ht] (immV [VAL_int32 i]) -∗
-          WP [AI_basic (BI_block tf es1)] @ s; E {{ w, Φ w }})) -∗
-      WP to_e_list (BI_const (VAL_int32 i) :: es) @ s; E {{ w, Φ w }}.
+         interp_val sr [RefT cap (LocP ptr GCMem) ht] (immV [VAL_int32 i]) -∗
+         WP [AI_basic (BI_block tf es2)] @ s; E {{ v, Φ v }}) ∧
+      ▷ (↪[frame] f -∗
+         interp_val sr [RefT cap (LocP ptr LinMem) ht] (immV [VAL_int32 i]) -∗
+         WP [AI_basic (BI_block tf es1)] @ s; E {{ v, Φ v }}) -∗
+      WP to_e_list (BI_const (VAL_int32 i) :: es) @ s; E {{ v, Φ v }}.
   Proof.
     intros Hcomp.
     unfold if_gc_bit in Hcomp.
@@ -115,17 +116,24 @@ Section CodeGen.
     split; first assumption.
     split; first assumption.
 
-    iIntros "Hfr Href Hif".
-  Abort.
+    iIntros "Hfr [Href | Href] Hif".
+  Admitted.
 
   (* TODO *)
-  Lemma wp_load_value_tagged s E get_offset ty wl wl' es :
-    run_codegen (load_value_tagged me fe get_offset ty) wl = inr (tt, wl', es) ->
-    ⊢ True -∗
-      WP to_e_list es @ s; E {{ w, ⌜w = immV []⌝ }}.
+  Lemma wp_load_value_tagged_struct s E cap ptr szs tys offset sz_off n_off ty wl wl' es idx a f :
+    tys !! idx = Some ty ->
+    struct_field_offset szs idx = inr sz_off ->
+    (* TODO: Are the sizes closed?
+             If so, how is it related to the Wasm args that get_offset uses? *)
+    eval_closed_size sz_off = Some (Wasm_int.nat_of_uint i32m n_off) ->
+    f.(f_locs) !! (localimm offset) = Some (VAL_int32 n_off) ->
+    run_codegen (load_value_tagged me fe offset ty) wl = inr (tt, wl', es) ->
+    ⊢ ↪[frame] f -∗
+      interp_val sr [RefT cap (LocP ptr GCMem) (StructType (zip tys szs))] (immV [VAL_int32 a]) ∨
+      interp_val sr [RefT cap (LocP ptr LinMem) (StructType (zip tys szs))] (immV [VAL_int32 a]) -∗
+      WP to_e_list es @ s; E {{ v, interp_val sr [ty] v }}.
   Proof.
-    intros Hcomp.
-    iIntros (HTrue).
+    intros Hty Hsz_off Hn_off Hoffset Hcomp.
     unfold load_value_tagged in Hcomp.
 
     apply run_codegen_bind_dist in Hcomp.
@@ -149,7 +157,19 @@ Section CodeGen.
     subst x3 wl3 es4 es5.
     clear Hcomp3.
 
-    iSimpl.
+    apply run_codegen_bind_dist in Hcomp4.
+    destruct Hcomp4 as ([[] []] & wl4 & es7 & es8 & Hcomp4 & Hcomp5 & Hes6).
+    cbn in Hcomp5.
+    inversion Hcomp5.
+    subst es6 es8 wl4.
+    clear Hcomp5.
+
+    apply wp_if_gc_bit with (s := s) (E := E) (cap := cap) (ptr := ptr) (i := a) (f := f)
+                            (ht := StructType (zip tys szs)) (Φ := interp_val sr [ty])
+      in Hcomp4.
+    destruct Hcomp4 as (wl5 & es9 & es10 & Hcomp5 & Hcomp6 & Hwp).
+
+    iIntros "Hf Href".
   Abort.
 
 End CodeGen.
